# 公式證明： 1+2+3+...+(n-2)+(n-1)+n = n(n+1)/2

`
1 + 2       + 3      +...+ (n-2) + (n-1) + n = S--------第1️式
`

把 第1式 倒過來寫，成 第2式：

`
n + (n-1)    + (n-2) +...+     3 + 2     + 1 = S--------第2式
`

第1式 加上 第2式：

`
(n+1) + [(n-1)+2] + [(n-2)+3] +...+ [(n-2)+3] + [(n-1)+2] + (n+1) = 2S
`

整理一下：

`
(n+1) + (n+1) + (n+1) +...+ (n+1) + (n+1) + (n+1) = 2S
`

總共有 n 個 (n+1)，所以進一步整理成：

`
n(n+1) = 2S
`

`
S = n(n+1)/2
`

ref: 維基百科 https://zh.m.wikipedia.org/wiki/1_%2B_2_%2B_3_%2B_4_%2B_%E2%80%A6

---

所以 1+2+3+...+(n-2)+(n-1)+n 的運算既可以寫成：

```csharp
public static decimal Sum(int[] numbers)
{
            int output= numbers[0];

            for(int i = 1; i < numbers.Length; ++i)
            {
                output +=  numbers[i];
            }

            return output;
}
```

或：

```csharp
using System.Linq;

public static decimal Sum(int[] numbers)
{
           return numbers.Sum();
}
```

或：

```csharp
public static decimal Sum(int[] numbers)
{
            return numbers.Length*(numbers.Length + 1) /2;
}
```
